rethinking how to state compile_val
want to be able to reuse a theorem that says if code is good for push,
then the same code appended by retbc is good for return. this should
then cover all the cases where the compiler generates the same code
(i.e. knows it's not going to jump).

compiler/correctness/compileCorrectnessScript.sml
@@ -2213,58 +2213,6 @@ val good_code_env_append = store_thm("good_code_env_append",
  res_tac >> rw[] >> metis_tac[APPEND_ASSOC])
 val _ = export_rewrites["good_code_env_append"]
 
-val code_for_push_def = Define`
-  code_for_push sm acc nl renv rsz code c d s env s' vs =
-    ∀bs bc0.
-      good_code_env c d bc0 ∧
-      (bs.code = bc0 ++ code) ∧
-      (bs.pc = next_addr bs.inst_length (bc0 ++ acc)) ∧
-      Cenv_bs c sm s env renv rsz (bs with code := (bc0 ++ acc)) ∧
-      ALL_DISTINCT (FILTER is_Label (bc0 ++ acc)) ∧
-      EVERY (combin$C $< nl o dest_Label) (FILTER is_Label (bc0 ++ acc))
-      ⇒
-      ∃bvs rf.
-      let bs' = bs with <| stack := (REVERSE bvs)++bs.stack; pc := next_addr bs.inst_length bs.code; refs := rf |> in
-      bc_next^* bs bs' ∧
-      EVERY2 (Cv_bv (mk_pp (DRESTRICT sm (FDOM s')) c bs')) vs bvs ∧
-      Cenv_bs c sm s' env renv (rsz+(LENGTH vs)) bs' ∧
-      DRESTRICT bs.refs (COMPL (FRANGE (DRESTRICT sm (FDOM s)))) ⊑ DRESTRICT rf (COMPL (FRANGE (DRESTRICT sm (FDOM s'))))`
-
-val code_for_return_def = Define`
-  code_for_return sm acc renv az code c d s env s' v =
-    ∀bs bc0 bc1 env0 ns defs xs vs benv ret args cl st.
-      (az = LENGTH args) ∧
-      (env = extend_rec_env env0 env0 ns defs xs vs) ∧
-      EVERY2 (Cv_bv (mk_pp (DRESTRICT sm (FDOM s)) c bs)) vs args ∧
-      Cenv_bs c sm s (DRESTRICT env (FDOM renv)) renv 0 bs ∧
-      (bs.code = bc0 ++ code ++ bc1) ∧
-      (bs.pc = next_addr bs.inst_length (bc0 ++ acc)) ∧
-      (bs.stack = benv::CodePtr ret::(REVERSE args)++cl::st)
-      ⇒
-      ∃bv rf.
-      let bs' = bs with <| stack := bv::st; pc := ret; refs := rf |> in
-      bc_next^* bs bs' ∧
-      Cv_bv (mk_pp (DRESTRICT sm (FDOM s')) c bs') v bv ∧
-      s_refs c sm s' bs' ∧
-      DRESTRICT bs.refs (COMPL (FRANGE (DRESTRICT sm (FDOM s)))) ⊑ DRESTRICT rf (COMPL (FRANGE (DRESTRICT sm (FDOM s'))))`
-
-(* TODO: move *)
-val EVERY2_THM = store_thm("EVERY2_THM",
-  ``(!P ys. EVERY2 P [] ys = (ys = [])) /\
-    (!P yys x xs. EVERY2 P (x::xs) yys = ?y ys. (yys = y::ys) /\ (P x y) /\ (EVERY2 P xs ys)) /\
-    (!P xs. EVERY2 P xs [] = (xs = [])) /\
-    (!P xxs y ys. EVERY2 P xxs (y::ys) = ?x xs. (xxs = x::xs) /\ (P x y) /\ (EVERY2 P xs ys))``,
-  REPEAT CONJ_TAC THEN GEN_TAC THEN TRY (
-    SRW_TAC[][EVERY2_EVERY,LENGTH_NIL] THEN
-    SRW_TAC[][EQ_IMP_THM] THEN NO_TAC ) THEN
-  Cases THEN SRW_TAC[][EVERY2_EVERY])
-val _ = export_rewrites["EVERY2_THM"]
-
-val with_same_refs = store_thm("with_same_refs",
-  ``(x with refs := x.refs) = x``,
-  rw[bc_state_component_equality])
-val _ = export_rewrites["with_same_refs"]
-
 val retbc_thm = store_thm("retbc_thm",
   ``∀bs bc0 bc1 bv vs benv ret args x st bs'.
     (bs.stack = bv::vs++benv::CodePtr ret::args++x::st) ∧
@@ -2328,35 +2276,135 @@ val retbc_thm = store_thm("retbc_thm",
   rw[bc_eval1_thm] >>
   rw[bc_eval1_def])
 
+(*
+val code_for_push_def = Define`
+  code_for_push sm acc nl renv rsz code c d s env s' vs =
+    ∀bs bc0 bc1.
+      (∃n. n ≤ LENGTH bs.code ∧ good_code_env c d (TAKE n bs.code)) ∧
+      (bs.code = bc0 ++ code ++ bc1) ∧
+      (bs.pc = next_addr bs.inst_length (bc0 ++ acc)) ∧
+      Cenv_bs c sm s env renv rsz (bs with code := (bc0 ++ acc)) ∧
+      ALL_DISTINCT (FILTER is_Label (bc0 ++ acc)) ∧
+      EVERY (combin$C $< nl o dest_Label) (FILTER is_Label (bc0 ++ acc))
+      ⇒
+      ∃bvs rf.
+      let bs' = bs with <| stack := (REVERSE bvs)++bs.stack; pc := next_addr bs.inst_length bs.code; refs := rf |> in
+      bc_next^* bs bs' ∧
+      EVERY2 (Cv_bv (mk_pp (DRESTRICT sm (FDOM s')) c bs')) vs bvs ∧
+      Cenv_bs c sm s' env renv (rsz+(LENGTH vs)) bs' ∧
+      DRESTRICT bs.refs (COMPL (FRANGE (DRESTRICT sm (FDOM s)))) ⊑ DRESTRICT rf (COMPL (FRANGE (DRESTRICT sm (FDOM s'))))`
+
+val code_for_return_def = Define`
+  code_for_return sm acc renv az code c d s env s' v =
+    ∀bs bc0 bc1 env0 ns defs xs vs benv ret args cl st.
+      (∃n. n ≤ LENGTH bs.code ∧ good_code_env c d (TAKE n bs.code)) ∧
+      (bs.code = bc0 ++ code ++ bc1) ∧
+      (bs.pc = next_addr bs.inst_length (bc0 ++ acc)) ∧
+      Cenv_bs c sm s (DRESTRICT env (FDOM renv)) renv 0 bs ∧
+      (az = LENGTH args) ∧
+      (env = extend_rec_env env0 env0 ns defs xs vs) ∧
+      EVERY2 (Cv_bv (mk_pp (DRESTRICT sm (FDOM s)) c bs)) vs args ∧
+      (bs.stack = benv::CodePtr ret::(REVERSE args)++cl::st)
+      ⇒
+      ∃bv rf.
+      let bs' = bs with <| stack := bv::st; pc := ret; refs := rf |> in
+      bc_next^* bs bs' ∧
+      Cv_bv (mk_pp (DRESTRICT sm (FDOM s')) c bs') v bv ∧
+      s_refs c sm s' bs' ∧
+      DRESTRICT bs.refs (COMPL (FRANGE (DRESTRICT sm (FDOM s)))) ⊑ DRESTRICT rf (COMPL (FRANGE (DRESTRICT sm (FDOM s'))))`
+*)
+
+(* TODO: move *)
+val EVERY2_THM = store_thm("EVERY2_THM",
+  ``(!P ys. EVERY2 P [] ys = (ys = [])) /\
+    (!P yys x xs. EVERY2 P (x::xs) yys = ?y ys. (yys = y::ys) /\ (P x y) /\ (EVERY2 P xs ys)) /\
+    (!P xs. EVERY2 P xs [] = (xs = [])) /\
+    (!P xxs y ys. EVERY2 P xxs (y::ys) = ?x xs. (xxs = x::xs) /\ (P x y) /\ (EVERY2 P xs ys))``,
+  REPEAT CONJ_TAC THEN GEN_TAC THEN TRY (
+    SRW_TAC[][EVERY2_EVERY,LENGTH_NIL] THEN
+    SRW_TAC[][EQ_IMP_THM] THEN NO_TAC ) THEN
+  Cases THEN SRW_TAC[][EVERY2_EVERY])
+val _ = export_rewrites["EVERY2_THM"]
+
+val with_same_refs = store_thm("with_same_refs",
+  ``(x with refs := x.refs) = x``,
+  rw[bc_state_component_equality])
+val _ = export_rewrites["with_same_refs"]
+
+val code_for_push_def = Define`
+  code_for_push sm bs bc0 code s s' c env vs renv rsz =
+    ∃bvs rf.
+    let bs' = bs with <| stack := (REVERSE bvs)++bs.stack; pc := next_addr bs.inst_length (bc0 ++ code); refs := rf |> in
+    bc_next^* bs bs' ∧
+    EVERY2 (Cv_bv (mk_pp (DRESTRICT sm (FDOM s')) c bs')) vs bvs ∧
+    Cenv_bs c sm s' env renv (rsz+(LENGTH vs)) bs' ∧
+    DRESTRICT bs.refs (COMPL (FRANGE (DRESTRICT sm (FDOM s)))) ⊑ DRESTRICT rf (COMPL (FRANGE (DRESTRICT sm (FDOM s'))))`
+
+val code_for_return_def = Define`
+  code_for_return sm bs st ret v s s' c =
+    ∃bv rf.
+    let bs' = bs with <| stack := bv::st; pc := ret; refs := rf |> in
+    bc_next^* bs bs' ∧
+    Cv_bv (mk_pp (DRESTRICT sm (FDOM s')) c bs') v bv ∧
+    s_refs c sm s' bs' ∧
+    DRESTRICT bs.refs (COMPL (FRANGE (DRESTRICT sm (FDOM s)))) ⊑ DRESTRICT rf (COMPL (FRANGE (DRESTRICT sm (FDOM s'))))`
+
+val code_for_push_return = store_thm("code_for_push_return",
+  ``∀sm acc nl sz code c d s env s' v az.
+    code_for_push sm bs bc0 code s s' c env vs renv rsz
+    ⇒
+    code_for_return sm bs st ret v s s' c
+
 val compile_val = store_thm("compile_val",
   ``(∀c d s env exp res. Cevaluate c d s env exp res ⇒
-      ∀sm s' v.
+      ∀sm s' v cs bs bc0 code bc1.
         Cexp_pred exp ∧
         DISJOINT (set (binders exp)) (FDOM env) ∧ ALL_DISTINCT (binders exp) ∧
         BIGUNION (IMAGE all_Clocs (FRANGE env)) ⊆ FDOM s ∧
         BIGUNION (IMAGE all_Clocs (FRANGE s)) ⊆ FDOM s ∧
         (res = (s', Rval v)) ∧
-        good_sm sm ∧ FDOM s' ⊆ FDOM sm ⇒
-      (∀cs.
+        good_sm sm ∧ FDOM s' ⊆ FDOM sm ∧
         good_ecs cs.ecs ∧ free_labs exp ⊆ FDOM cs.ecs ∧
-        (cs.tail = TCNonTail) ∧ (cs.decl = NONE) ⇒
-        code_for_push sm (REVERSE cs.out) cs.next_label cs.env cs.sz (REVERSE (compile cs exp).out) c d s env s' [v]) ∧
-      (∀cs az.
-        (cs.tail = TCTail az 0) ∧ (cs.sz = 0) ∧ (cs.decl = NONE) ∧ (free_vars c exp ⊆ FDOM cs.env) ⇒
+        (∃n. n ≤ LENGTH bs.code ∧ good_code_env c d (TAKE n bs.code)) ∧
+        (bs.code = bc0 ++ code ++ bc1) ∧
+        (bs.pc = next_addr bs.inst_length (bc0 ++ (REVERSE cs.out))) ∧
+        (free_vars c exp ⊆ FDOM cs.env) ∧
+        Cenv_bs c sm s (DRESTRICT env (FDOM cs.env)) cs.env cs.sz bs ∧
+        ALL_DISTINCT (FILTER is_Label (bc0 ++ REVERSE cs.out)) ∧
+        EVERY (combin$C $< cs.next_label o dest_Label) (FILTER is_Label (bc0 ++ REVERSE cs.out))
+        ⇒
+      ((cs.tail = TCNonTail) ∧ (cs.decl = NONE) ∧ (code = REVERSE (compile cs exp).out) ⇒
+        code_for_push sm bs bc0 code s s' c env [v] cs.env cs.sz) ∧
+      (∀az.
         let cs1 = compile cs exp in let n = case cs1.tail of TCTail j k => k+1 in
-        code_for_return sm (REVERSE cs.out) cs.env az ((REVERSE cs1.out)++(retbc n az)) c d s env s' v)) ∧
+        (cs.tail = TCTail az 0) ∧ (cs.sz = 0) ∧ (cs.decl = NONE) ∧
+        (code = ((REVERSE cs1.out)++(retbc n az))) ⇒
+        ∀env0 ns defs xs vs benv ret args cl st.
+        (az = LENGTH args) ∧
+        (env = extend_rec_env env0 env0 ns defs xs vs) ∧
+        EVERY2 (Cv_bv (mk_pp (DRESTRICT sm (FDOM s)) c bs)) vs args ∧
+        (bs.stack = benv::CodePtr ret::(REVERSE args)++cl::st)
+        ⇒
+        code_for_return sm bs st ret v s s' c)) ∧
     (∀c d s env exps ress. Cevaluate_list c d s env exps ress ⇒
-      ∀sm s' vs.
+      ∀sm s' vs cs bs bc0 code bc1.
         EVERY Cexp_pred exps ∧
         DISJOINT (set (FLAT (MAP binders exps))) (FDOM env) ∧ ALL_DISTINCT (FLAT (MAP binders exps)) ∧
         BIGUNION (IMAGE all_Clocs (FRANGE env)) ⊆ FDOM s ∧
         BIGUNION (IMAGE all_Clocs (FRANGE s)) ⊆ FDOM s ∧
         (ress = (s', Rval vs)) ∧
-        good_sm sm ∧ FDOM s' ⊆ FDOM sm ⇒
-      (∀cs.
+        good_sm sm ∧ FDOM s' ⊆ FDOM sm ∧
         good_ecs cs.ecs ∧ free_labs_list exps ⊆ FDOM cs.ecs ∧
-        (cs.tail = TCNonTail) ∧ (cs.decl = NONE) ⇒
-        code_for_push sm (REVERSE cs.out) cs.next_label cs.env cs.sz (REVERSE (FOLDL compile cs exps).out) c d s env s' vs))``,
+        (∃n. n ≤ LENGTH bs.code ∧ good_code_env c d (TAKE n bs.code)) ∧
+        (bs.code = bc0 ++ code ++ bc1) ∧
+        (bs.pc = next_addr bs.inst_length (bc0 ++ (REVERSE cs.out))) ∧
+        (BIGUNION (IMAGE (free_vars c) (set exps)) ⊆ FDOM cs.env) ∧
+        Cenv_bs c sm s (DRESTRICT env (FDOM cs.env)) cs.env cs.sz bs ∧
+        ALL_DISTINCT (FILTER is_Label (bc0 ++ REVERSE cs.out)) ∧
+        EVERY (combin$C $< cs.next_label o dest_Label) (FILTER is_Label (bc0 ++ REVERSE cs.out))
+        ⇒
+      ((cs.tail = TCNonTail) ∧ (cs.decl = NONE) ∧ (code = REVERSE (FOLDL compile cs exps).out) ⇒
+        code_for_push sm bs bc0 code s s' c env vs cs.env cs.sz))``,
   ho_match_mp_tac Cevaluate_strongind >>
   strip_tac >- rw[] >>
   strip_tac >- rw[] >>
@@ -2364,7 +2412,7 @@ val compile_val = store_thm("compile_val",
   strip_tac >- rw[] >>
   strip_tac >- (
     ntac 4 gen_tac >> qx_gen_tac`n` >> strip_tac >> simp[] >>
-    qx_gen_tac`sm` >> strip_tac >>
+    rpt gen_tac >> strip_tac >>
     conj_tac >- (
       rw[code_for_push_def,compile_def,Cenv_bs_def,fmap_rel_def] >>
       first_assum (qspec_then `n` mp_tac) >>
@@ -2467,14 +2515,18 @@ val compile_val = store_thm("compile_val",
     srw_tac[ARITH_ss][bump_pc_def,Abbr`ls0`,FILTER_APPEND,SUM_APPEND,ADD1] >>
     rw[bc_state_component_equality]))) >>
   strip_tac >- (
-
-    rw[compile_def,LET_THM] >>
+    fsrw_tac[ETA_ss][FOLDL_UNION_BIGUNION] >>
+    rpt gen_tac >> strip_tac >>
+    rpt gen_tac >> strip_tac >>
+    simp[compile_def,LET_THM] >>
     fsrw_tac[ETA_ss][] >>
     first_x_assum (qspec_then`sm`mp_tac) >> simp[] >>
     qabbrev_tac`cs0 = cs with <| tail := TCNonTail; decl := NONE|>` >>
     disch_then(qspec_then`cs0`mp_tac) >>
     simp[Abbr`cs0`] >>
-    simp[code_for_push_def] >>
+
+    simp[code_for_push_def,code_for_return_def] >>
+
     srw_tac[DNF_ss][Once Cv_bv_cases] >>
     qmatch_assum_abbrev_tac `bs.code = ls0 ++ [x]` >>
     first_x_assum (qspecl_then [`bs with code := ls0`,`bc0`] mp_tac) >>
